src/Init/Data/Option/Basic.lean
@@ -212,6 +212,9 @@ instance (α) [BEq α] [LawfulBEq α] : LawfulBEq (Option α) where
 @[simp] theorem all_none : Option.all p none = true := rfl
 @[simp] theorem all_some : Option.all p (some x) = p x := rfl
 
+@[simp] theorem any_none : Option.any p none = false := rfl
+@[simp] theorem any_some : Option.any p (some x) = p x := rfl
+
 /-- The minimum of two optional values. -/
 protected def min [Min α] : Option α → Option α → Option α
   | some x, some y => some (Min.min x y)
